Rename `Steps` to `Multistep`

Stlc/Step.lean
@@ -11,9 +11,9 @@ local infixr:10 " ⟶ " => Step
 
 open Term Syntax in
 inductive Step : Term → Term → Prop
-| app_cont {x τ t v} : Value v → (t[(λ x : τ, t) v] ⟶ t[[x := v] t])
+| app_cont {τ t₁ t₂ x} : Value t₂ → (t[(λ x : τ, t₁) t₂] ⟶ t[[x := t₂] t₁])
 | app_cong_l {t₁ t₁' t₂} : (t₁ ⟶ t₁') → (t[t₁ t₂] ⟶ t[t₁' t₂])
-| app_cong_r {v t t'} : Value v → (t ⟶ t') → (t[v t] ⟶ t[v t'])
+| app_cong_r {t₁ t₂ t₂'} : Value t₁ → (t₂ ⟶ t₂') → (t[t₁ t₂] ⟶ t[t₁ t₂'])
 | ite_cont_true {t₁ t₂} : t[if true then t₁ else t₂] ⟶ t₁
 | ite_cont_false {t₁ t₂} : t[if false then t₁ else t₂] ⟶ t₂
 | ite_cong {t₁ t₁' t₂ t₃} :
@@ -23,38 +23,41 @@ end
 
 infixr:10 " ⟶ " => Step
 
-def Steps := Relation.ReflTransGen Step
+def Multistep := Relation.ReflTransGen Step
 
-infixr:10 " ⟶* " => Steps
+infixr:10 " ⟶* " => Multistep
 
 @[refl]
-theorem Steps.refl {t : Term} : t ⟶* t := Relation.ReflTransGen.refl
+theorem Multistep.refl {t : Term} : t ⟶* t :=
+  Relation.ReflTransGen.refl
 
 @[trans]
-theorem Steps.trans {t₁ t₂ t₃ : Term} : (t₁ ⟶* t₂) → (t₂ ⟶* t₃) → (t₁ ⟶* t₃) :=
+theorem Multistep.trans {t₁ t₂ t₃ : Term} : (t₁ ⟶* t₂) → (t₂ ⟶* t₃) → (t₁ ⟶* t₃) :=
   Relation.ReflTransGen.trans
 
-theorem Steps.head {t₁ t₂ t₃ : Term} : (t₁ ⟶ t₂) → (t₂ ⟶* t₃) → (t₁ ⟶* t₃) :=
+theorem Multistep.head {t₁ t₂ t₃ : Term} : (t₁ ⟶ t₂) → (t₂ ⟶* t₃) → (t₁ ⟶* t₃) :=
   Relation.ReflTransGen.head
 
-theorem Steps.tail {t₁ t₂ t₃ : Term} : (t₁ ⟶* t₂) → (t₂ ⟶ t₃) → (t₁ ⟶* t₃) :=
+theorem Multistep.tail {t₁ t₂ t₃ : Term} : (t₁ ⟶* t₂) → (t₂ ⟶ t₃) → (t₁ ⟶* t₃) :=
   Relation.ReflTransGen.tail
 
-theorem Steps.single {t₁ t₂ : Term} : (t₁ ⟶ t₂) → (t₁ ⟶* t₂) := Relation.ReflTransGen.single
+theorem Multistep.single {t₁ t₂ : Term} : (t₁ ⟶ t₂) → (t₁ ⟶* t₂) :=
+  Relation.ReflTransGen.single
 
-theorem Term.Value.no_step {v t : Term} : Value v → ¬(v ⟶ t) := by
+theorem Term.Value.no_step {t t' : Term} : Value t → ¬(t ⟶ t') := by
   rintro ⟨⟩ <;> rintro ⟨⟩
 
 theorem Step.not_value {t t' : Term} : (t ⟶ t') → ¬t.Value := by
   rintro ⟨⟩ <;> rintro ⟨⟩
 
 open Syntax in
+@[simp]
 def Term.step : Term → Option Term
 | t[(λ x : τ, t₁) t₂] =>
-    if Value t₂ then subst x t₂ t₁ else t₂.step.map <| .app (.abs x τ t₁)
-| t[t₁ t₂] => if Value t₁ then t₂.step.map (.app t₁) else t₁.step.map (.app · t₂)
+    if Value t₂ then subst x t₂ t₁ else t₂.step.map <| app (abs x τ t₁)
+| t[t₁ t₂] => if Value t₁ then t₂.step.map (app t₁) else t₁.step.map (app · t₂)
 | t[if true then t else _] | t[if false then _ else t] => t
-| t[if t₁ then t₂ else t₃] => t₁.step.map (.ite · t₂ t₃)
+| t[if t₁ then t₂ else t₃] => t₁.step.map (ite · t₂ t₃)
 | _ => none
 
 theorem Term.step_iff_step (t t' : Term) : t.step = some t' ↔ (t ⟶ t') := by
@@ -106,11 +109,11 @@ instance : DecidableRel Step := fun t₁ t₂ =>
   decidable_of_decidable_of_iff <| Term.step_iff_step t₁ t₂
 
 theorem Term.not_step_iff_not_step (t : Term) : t.step = none ↔ ∀ t', ¬(t ⟶ t') := by
-  simp [←Term.step_iff_step]
+  simp_rw [←step_iff_step]
   constructor <;> intro h
-  · simp only [h, reduceCtorEq, not_false_eq_true, implies_true]
+  · simp [h]
   · ext
-    simp only [h, reduceCtorEq]
+    simp [h]
 
 def Term.step_n : Term → Nat → Term
 | x, 0 => x
@@ -127,13 +130,13 @@ theorem Term.step_n_spec (t : Term) (n : Nat) : t ⟶* t.step_n n := by
     rw [step_n]
     by_cases h : ∃ t', t.step_n n ⟶ t'
     · rcases h with ⟨_, h'⟩
-      simp only [(Term.step_iff_step ..).mpr h']
+      simp only [(step_iff_step ..).mpr h']
       rcases (ih t).cases_head with ht | _
       · rw [ht]
-        exact Steps.single h'
-      · exact Steps.tail (ih t) h'
+        exact Multistep.single h'
+      · exact Multistep.tail (ih t) h'
     · push_neg at h
-      rw [←Term.not_step_iff_not_step] at h
+      rw [←not_step_iff_not_step] at h
       rw [h]
       exact ih t
 
@@ -149,7 +152,7 @@ theorem Step.unique {t t₁ t₂} : (t ⟶ t₁) → (t ⟶ t₂) → t₁ = t�
     | app_cong_l h₃ => cases h₃
     | app_cong_r _ h₃ => cases v.no_step h₃
   | app_cong_l h₃ ih => cases h₂ with
-    | app_cont => cases (Term.Value.abs ..).no_step h₃
+    | app_cont => cases h₃
     | app_cong_l h₄ => rw [ih h₄]
     | app_cong_r v => cases v.no_step h₃
   | app_cong_r v h₃ ih => cases h₂ with
@@ -163,17 +166,16 @@ theorem Step.unique {t t₁ t₂} : (t ⟶ t₁) → (t ⟶ t₂) → t₁ = t�
     | ite_cont_false => rfl
     | ite_cong h₃ => cases Term.Value.false.no_step h₃
   | ite_cong h₃ ih => cases h₂ with
-    | ite_cont_true => cases Term.Value.true.no_step h₃
-    | ite_cont_false => cases Term.Value.false.no_step h₃
+    | ite_cont_true | ite_cont_false => cases h₃
     | ite_cong h₄ => rw [ih h₄]
 
-theorem Steps.cont_iff {t₁ t₂ v : Term} (hv : v.Value) (h : t₁ ⟶ t₂) :
-    (t₁ ⟶* v) ↔ (t₂ ⟶* v) := by
+theorem Multistep.cont_iff {t t₁ t₂ : Term} (ht : t.Value) (h : t₁ ⟶ t₂) :
+    (t₁ ⟶* t) ↔ (t₂ ⟶* t) := by
   constructor
   · intro h₂
     obtain rfl | ⟨_, h₃, _⟩ := h₂.cases_head
-    · cases hv.no_step h
+    · cases ht.no_step h
     · rwa [h.unique h₃]
-  · exact Steps.head h
+  · exact head h
 
 end Stlc
